Adapted to new inductive definition package.

thys/Abstract-Hoare-Logics/Proc/PHoareTotal.thy
@@ -1,5 +1,5 @@
 (*  Title:      Inductive definition of Hoare logic for total correctness
-    ID:         $Id: PHoareTotal.thy,v 1.2 2006-11-17 01:28:44 makarius Exp $
+    ID:         $Id: PHoareTotal.thy,v 1.3 2007-07-11 10:05:49 stefanberghofer Exp $
     Author:      Tobias Nipkow, 2001/2006
     Maintainer:  Tobias Nipkow
 *)
@@ -18,40 +18,37 @@ constdefs
             ("(_ /\<Turnstile>\<^sub>t {(1_)}/ (_)/ {(1_))}" 50)
  "C \<Turnstile>\<^sub>t {P}c{Q}  \<equiv>  (\<forall>(P',c',Q') \<in> C. \<Turnstile>\<^sub>t {P'}c'{Q'}) \<longrightarrow> \<Turnstile>\<^sub>t {P}c{Q}"
 
-consts thoare :: "('a cntxt \<times> 'a assn \<times> com \<times> 'a assn) set"
-abbreviation hoare1 :: "'a cntxt \<Rightarrow> 'a assn \<times> com \<times> 'a assn \<Rightarrow> bool" ("_ \<turnstile>\<^sub>t _") where
-  "C \<turnstile>\<^sub>t x \<equiv> (C,x) \<in> thoare"
-abbreviation
- thoare3 :: "'a cntxt \<Rightarrow> 'a assn \<Rightarrow> com \<Rightarrow> 'a assn \<Rightarrow> bool"
-                   ("(_ \<turnstile>\<^sub>t/ ({(1_)}/ (_)/ {(1_)}))" [50,0,0,0] 50) where
- "C \<turnstile>\<^sub>t {P}c{Q}  \<equiv> (C,P,c,Q) : thoare"
 
-
-inductive thoare
-intros
+inductive
+  thoare :: "'a cntxt \<Rightarrow> 'a assn \<Rightarrow> com \<Rightarrow> 'a assn \<Rightarrow> bool"
+   ("(_ \<turnstile>\<^sub>t/ ({(1_)}/ (_)/ {(1_)}))" [50,0,0,0] 50)
+where
   Do: "C \<turnstile>\<^sub>t {\<lambda>z s. (\<forall>t \<in> f s . P z t) \<and> f s \<noteq> {}} Do f {P}"
-  Semi: "\<lbrakk> C \<turnstile>\<^sub>t {P}c1{Q}; C \<turnstile>\<^sub>t {Q}c2{R} \<rbrakk> \<Longrightarrow> C \<turnstile>\<^sub>t {P} c1;c2 {R}"
-  If: "\<lbrakk> C \<turnstile>\<^sub>t {\<lambda>z s. P z s \<and> b s}c{Q}; C \<turnstile>\<^sub>t {\<lambda>z s. P z s \<and> ~b s}d{Q}  \<rbrakk> \<Longrightarrow>
+| Semi: "\<lbrakk> C \<turnstile>\<^sub>t {P}c1{Q}; C \<turnstile>\<^sub>t {Q}c2{R} \<rbrakk> \<Longrightarrow> C \<turnstile>\<^sub>t {P} c1;c2 {R}"
+| If: "\<lbrakk> C \<turnstile>\<^sub>t {\<lambda>z s. P z s \<and> b s}c{Q}; C \<turnstile>\<^sub>t {\<lambda>z s. P z s \<and> ~b s}d{Q}  \<rbrakk> \<Longrightarrow>
       C \<turnstile>\<^sub>t {P} IF b THEN c ELSE d {Q}"
-  While:
+| While:
   "\<lbrakk>wf r;  \<forall>s'. C \<turnstile>\<^sub>t {\<lambda>z s. P z s \<and> b s \<and> s' = s} c {\<lambda>z s. P z s \<and> (s,s') \<in> r}\<rbrakk>
    \<Longrightarrow> C \<turnstile>\<^sub>t {P} WHILE b DO c {\<lambda>z s. P z s \<and> \<not>b s}"
 
-Call:
+| Call:
   "\<lbrakk>wf r;  \<forall>s'. {(\<lambda>z s. P z s \<and> (s,s') \<in> r, CALL, Q)}
                  \<turnstile>\<^sub>t {\<lambda>z s. P z s \<and> s = s'} body {Q}\<rbrakk>
    \<Longrightarrow> {} \<turnstile>\<^sub>t {P} CALL {Q}"
 
-  Asm: "{(P,CALL,Q)} \<turnstile>\<^sub>t {P} CALL {Q}"
+| Asm: "{(P,CALL,Q)} \<turnstile>\<^sub>t {P} CALL {Q}"
 
-Conseq:
+| Conseq:
   "\<lbrakk> C \<turnstile>\<^sub>t {P'}c{Q'};
      (\<forall>s t. (\<forall>z. P' z s \<longrightarrow> Q' z t) \<longrightarrow> (\<forall>z. P z s \<longrightarrow> Q z t)) \<and>
      (\<forall>s. (\<exists>z. P z s) \<longrightarrow> (\<exists>z. P' z s)) \<rbrakk>
    \<Longrightarrow> C \<turnstile>\<^sub>t {P}c{Q}"
 
-  Local: "\<lbrakk> \<forall>s'. C \<turnstile>\<^sub>t {\<lambda>z s. P z s' \<and> s = f s'} c {\<lambda>z t. Q z (g s' t)} \<rbrakk> \<Longrightarrow>
+| Local: "\<lbrakk> \<forall>s'. C \<turnstile>\<^sub>t {\<lambda>z s. P z s' \<and> s = f s'} c {\<lambda>z t. Q z (g s' t)} \<rbrakk> \<Longrightarrow>
         C \<turnstile>\<^sub>t {P} LOCAL f;c;g {Q}"
+
+abbreviation hoare1 :: "'a cntxt \<Rightarrow> 'a assn \<times> com \<times> 'a assn \<Rightarrow> bool" ("_ \<turnstile>\<^sub>t _") where
+  "C \<turnstile>\<^sub>t x \<equiv> C \<turnstile>\<^sub>t {fst x}fst (snd x){snd (snd x)}"
 
 
 text{* The side condition in our rule of consequence looks quite different
@@ -146,18 +143,18 @@ declare MGT\<^isub>t_def[simp]
 
 lemma MGT_implies_complete:
  "{} \<turnstile>\<^sub>t MGT\<^isub>t c \<Longrightarrow> {} \<Turnstile>\<^sub>t {P}c{Q} \<Longrightarrow> {} \<turnstile>\<^sub>t {P}c{Q::state assn}";
-apply(unfold MGT\<^isub>t_def)
+apply(simp add: MGT\<^isub>t_def)
 apply (erule thoare.Conseq)
 apply(simp add: tvalid_defs)
 apply blast
 done
 
 lemma while_termiE: "\<lbrakk> WHILE b DO c \<down> s; b s \<rbrakk> \<Longrightarrow> c \<down> s"
-by(erule termi.elims, auto)
+by(erule termi.cases, auto)
 
 lemma while_termiE2:
   "\<lbrakk> WHILE b DO c \<down> s; b s; s -c\<rightarrow> t \<rbrakk> \<Longrightarrow> WHILE b DO c \<down> t"
-by(erule termi.elims, auto)
+by(erule termi.cases, auto)
 
 lemma MGT_lemma: "C \<turnstile>\<^sub>t MGT\<^isub>t CALL \<Longrightarrow> C \<turnstile>\<^sub>t MGT\<^isub>t c"
 apply (simp)
@@ -195,45 +192,41 @@ apply(fast intro: rtrancl_refl)
 done
 
 
-consts  exec1 :: "((com list \<times> state) \<times> (com list \<times> state))set"
-syntax
- "@exec1" :: "(com list \<times> state) \<Rightarrow> (com list \<times> state) \<Rightarrow> bool"  ("_ \<rightarrow> _" [81,81] 100)
- "@exec*" :: "(com list \<times> state) \<Rightarrow> (com list \<times> state) \<Rightarrow> bool"   ("_ \<rightarrow>\<^sup>* _" [81,81] 100)
+inductive_set
+  exec1 :: "((com list \<times> state) \<times> (com list \<times> state))set"
+  and exec1' :: "(com list \<times> state) \<Rightarrow> (com list \<times> state) \<Rightarrow> bool"  ("_ \<rightarrow> _" [81,81] 100)
+where
+  "cs0 \<rightarrow> cs1 \<equiv> (cs0,cs1) : exec1"
 
-translations
-  "cs0 \<rightarrow> cs1"	     == "(cs0,cs1) : exec1"
-  "cs0 \<rightarrow> (c1,s1)"  == "(cs0,c1,s1) : exec1"
+| Do[iff]: "t \<in> f s \<Longrightarrow> ((Do f)#cs,s) \<rightarrow> (cs,t)"
 
-  "cs0 \<rightarrow>\<^sup>* cs1" 	    == "(cs0,cs1) : exec1^*"
-  "cs0 \<rightarrow>\<^sup>* (c1,s1)" == "(cs0,c1,s1) : exec1^*"
+| Semi[iff]: "((c1;c2)#cs,s) \<rightarrow> (c1#c2#cs,s)"
 
-inductive exec1
-intros
-Do[iff]: "t \<in> f s \<Longrightarrow> ((Do f)#cs,s) \<rightarrow> (cs,t)"
+| IfTrue:   "b s \<Longrightarrow> ((IF b THEN c1 ELSE c2)#cs,s) \<rightarrow> (c1#cs,s)"
+| IfFalse: "\<not>b s \<Longrightarrow> ((IF b THEN c1 ELSE c2)#cs,s) \<rightarrow> (c2#cs,s)"
 
-Semi[iff]: "((c1;c2)#cs,s) \<rightarrow> (c1#c2#cs,s)"
+| WhileFalse: "\<not>b s \<Longrightarrow> ((WHILE b DO c)#cs,s) \<rightarrow> (cs,s)"
+| WhileTrue:   "b s \<Longrightarrow> ((WHILE b DO c)#cs,s) \<rightarrow> (c#(WHILE b DO c)#cs,s)"
 
-IfTrue:   "b s \<Longrightarrow> ((IF b THEN c1 ELSE c2)#cs,s) \<rightarrow> (c1#cs,s)"
-IfFalse: "\<not>b s \<Longrightarrow> ((IF b THEN c1 ELSE c2)#cs,s) \<rightarrow> (c2#cs,s)"
+| Call[iff]: "(CALL#cs,s) \<rightarrow> (body#cs,s)"
 
-WhileFalse: "\<not>b s \<Longrightarrow> ((WHILE b DO c)#cs,s) \<rightarrow> (cs,s)"
-WhileTrue:   "b s \<Longrightarrow> ((WHILE b DO c)#cs,s) \<rightarrow> (c#(WHILE b DO c)#cs,s)"
+| Local[iff]: "((LOCAL f;c;g)#cs,s) \<rightarrow> (c # Do(\<lambda>t. {g s t})#cs, f s)"
 
-Call[iff]: "(CALL#cs,s) \<rightarrow> (body#cs,s)"
-
-Local[iff]: "((LOCAL f;c;g)#cs,s) \<rightarrow> (c # Do(\<lambda>t. {g s t})#cs, f s)"
+abbreviation
+  exectr :: "(com list \<times> state) \<Rightarrow> (com list \<times> state) \<Rightarrow> bool"   ("_ \<rightarrow>\<^sup>* _" [81,81] 100)
+  where "cs0 \<rightarrow>\<^sup>* cs1 \<equiv> (cs0,cs1) : exec1^*"
 
 inductive_cases exec1E[elim!]:
- "([],s) \<rightarrow> u"
- "(Do f#cs,s) \<rightarrow> u"
- "((c1;c2)#cs,s) \<rightarrow> u"
- "((IF b THEN c1 ELSE c2)#cs,s) \<rightarrow> u"
- "((WHILE b DO c)#cs,s) \<rightarrow> u"
- "(CALL#cs,s) \<rightarrow> u"
- "((LOCAL f;c;g)#cs,s) \<rightarrow> u"
+ "([],s) \<rightarrow> (cs',s')"
+ "(Do f#cs,s) \<rightarrow> (cs',s')"
+ "((c1;c2)#cs,s) \<rightarrow> (cs',s')"
+ "((IF b THEN c1 ELSE c2)#cs,s) \<rightarrow> (cs',s')"
+ "((WHILE b DO c)#cs,s) \<rightarrow> (cs',s')"
+ "(CALL#cs,s) \<rightarrow> (cs',s')"
+ "((LOCAL f;c;g)#cs,s) \<rightarrow> (cs',s')"
 
 lemma [iff]: "\<not> ([],s) \<rightarrow> u"
-by blast
+by (induct u) blast
 
 lemma app_exec: "(cs,s) \<rightarrow> (cs',s') \<Longrightarrow> (cs@cs2,s) \<rightarrow> (cs'@cs2,s')"
 apply(erule exec1.induct)
@@ -260,15 +253,11 @@ apply(erule exec.induct)
 apply(blast intro: rtrancl_trans)
 done
 
-consts execs :: "(state \<times> com list \<times> state) set"
-abbreviation
-  execs' :: "state \<Rightarrow> com list \<Rightarrow> state \<Rightarrow> bool"   ("_/ =_\<Rightarrow>/ _" [50,0,50] 50) where
- "s =cs\<Rightarrow> t  \<equiv>  (s,cs,t) \<in> execs"
-
-inductive execs
-intros
-"s =[]\<Rightarrow> s"
-"s -c\<rightarrow> t \<Longrightarrow> t =cs\<Rightarrow> u \<Longrightarrow> s =c#cs\<Rightarrow> u"
+inductive
+  execs :: "state \<Rightarrow> com list \<Rightarrow> state \<Rightarrow> bool"   ("_/ =_\<Rightarrow>/ _" [50,0,50] 50)
+where
+  "s =[]\<Rightarrow> s"
+| "s -c\<rightarrow> t \<Longrightarrow> t =cs\<Rightarrow> u \<Longrightarrow> s =c#cs\<Rightarrow> u"
 
 inductive_cases [elim!]:
  "s =[]\<Rightarrow> t"
@@ -277,7 +266,7 @@ inductive_cases [elim!]:
 theorem exec1s_impl_execs: "(cs,s) \<rightarrow>\<^sup>* ([],t) \<Longrightarrow> s =cs\<Rightarrow> t"
 apply(erule converse_rtrancl_induct2)
  apply(rule execs.intros)
-apply(erule exec1.elims)
+apply(erule exec1.cases)
 apply(blast intro:execs.intros)
 apply(blast intro:execs.intros)
 apply(fastsimp intro:execs.intros)
@@ -366,6 +355,7 @@ apply(unfold inf_def)
 apply clarify
 apply(frule_tac x = 0 in spec)
 apply(erule_tac x = 1 in allE)
+apply(case_tac "fa (Suc 0)")
 apply clarsimp
 done
 
@@ -375,6 +365,7 @@ apply(rule iffI)
 apply clarify
 apply(rule_tac x = "\<lambda>i. f(Suc i)" in exI)
 apply(frule_tac x = 0 in spec)
+apply(case_tac "f (Suc 0)")
 apply clarsimp
 apply clarify
 apply(rule_tac x = "\<lambda>i. case i of 0 \<Rightarrow> ((c1;c2)#cs,s) | Suc i \<Rightarrow> f i" in exI)
@@ -387,6 +378,7 @@ apply(unfold inf_def)
 apply(rule iffI)
  apply clarsimp
  apply(frule_tac x = 0 in spec)
+ apply (case_tac "f (Suc 0)")
  apply(rule conjI)
   apply clarsimp
   apply(rule_tac x = "\<lambda>i. f(Suc i)" in exI)
@@ -406,6 +398,7 @@ apply(unfold inf_def)
 apply(rule iffI)
  apply clarsimp
  apply(frule_tac x = 0 in spec)
+ apply (case_tac "f (Suc 0)")
  apply(rule conjI)
   apply clarsimp
   apply(rule_tac x = "\<lambda>i. f(Suc i)" in exI)
@@ -425,6 +418,7 @@ apply(unfold inf_def)
 apply(rule iffI)
  apply clarsimp
  apply(frule_tac x = 0 in spec)
+ apply (case_tac "f (Suc 0)")
  apply clarsimp
  apply(rule_tac x = "\<lambda>i. f(Suc i)" in exI)
  apply clarsimp
@@ -440,6 +434,7 @@ apply(rule iffI)
  apply clarsimp
  apply(rename_tac F)
  apply(frule_tac x = 0 in spec)
+ apply (case_tac "F (Suc 0)")
  apply clarsimp
  apply(rule_tac x = "\<lambda>i. F(Suc i)" in exI)
  apply clarsimp
