thys/Abstract-Hoare-Logics/Procs/PsLang.thy
@@ -1,5 +1,5 @@
 (*  Title:       Mutually recursive procedures
-    ID:          $Id: PsLang.thy,v 1.2 2006-11-17 01:28:44 makarius Exp $
+    ID:          $Id: PsLang.thy,v 1.3 2007-07-11 10:05:49 stefanberghofer Exp $
     Author:      Tobias Nipkow, 2001/2006
     Maintainer:  Tobias Nipkow
 *)
@@ -37,91 +37,83 @@ the name of the procedure that is to be called.
 \end{itemize}
 *}
 
-consts  exec    :: "(state \<times> com \<times> state)set"
-abbreviation
- exec' :: "state \<Rightarrow> com \<Rightarrow> state \<Rightarrow> bool"   ("_/ -_\<rightarrow>/ _" [50,0,50] 50) where
- "s0 -c\<rightarrow> s1  \<equiv>  (s0,c,s1) \<in> exec"
-
-inductive exec
-intros
+inductive
+  exec :: "state \<Rightarrow> com \<Rightarrow> state \<Rightarrow> bool"   ("_/ -_\<rightarrow>/ _" [50,0,50] 50)
+where
     Do:     "t \<in> f s \<Longrightarrow> s -Do f\<rightarrow> t"
 
-    Semi:   "\<lbrakk> s0 -c1\<rightarrow> s1; s1 -c2\<rightarrow> s2 \<rbrakk> \<Longrightarrow> s0 -c1;c2\<rightarrow> s2"
+  | Semi:   "\<lbrakk> s0 -c1\<rightarrow> s1; s1 -c2\<rightarrow> s2 \<rbrakk> \<Longrightarrow> s0 -c1;c2\<rightarrow> s2"
 
-    IfTrue:  "\<lbrakk> b s;  s -c1\<rightarrow> t \<rbrakk> \<Longrightarrow> s -IF b THEN c1 ELSE c2\<rightarrow> t"
-    IfFalse: "\<lbrakk> \<not>b s; s -c2\<rightarrow> t \<rbrakk> \<Longrightarrow> s -IF b THEN c1 ELSE c2\<rightarrow> t"
+  | IfTrue:  "\<lbrakk> b s;  s -c1\<rightarrow> t \<rbrakk> \<Longrightarrow> s -IF b THEN c1 ELSE c2\<rightarrow> t"
+  | IfFalse: "\<lbrakk> \<not>b s; s -c2\<rightarrow> t \<rbrakk> \<Longrightarrow> s -IF b THEN c1 ELSE c2\<rightarrow> t"
 
-    WhileFalse: "\<not>b s \<Longrightarrow> s -WHILE b DO c\<rightarrow> s"
-    WhileTrue:  "\<lbrakk> b s; s -c\<rightarrow> t; t -WHILE b DO c\<rightarrow> u \<rbrakk>
+  | WhileFalse: "\<not>b s \<Longrightarrow> s -WHILE b DO c\<rightarrow> s"
+  | WhileTrue:  "\<lbrakk> b s; s -c\<rightarrow> t; t -WHILE b DO c\<rightarrow> u \<rbrakk>
                 \<Longrightarrow> s -WHILE b DO c\<rightarrow> u"
 
-    Call: "s -body p\<rightarrow> t \<Longrightarrow> s -CALL p\<rightarrow> t"
+  | Call: "s -body p\<rightarrow> t \<Longrightarrow> s -CALL p\<rightarrow> t"
 
-    Local: "f s -c\<rightarrow> t \<Longrightarrow> s -LOCAL f; c; g\<rightarrow> g s t"
+  | Local: "f s -c\<rightarrow> t \<Longrightarrow> s -LOCAL f; c; g\<rightarrow> g s t"
 
 lemma [iff]: "(s -Do f\<rightarrow> t) = (t \<in> f s)"
-by(auto elim: exec.elims intro:exec.intros)
+by(auto elim: exec.cases intro:exec.intros)
 
 lemma [iff]: "(s -c;d\<rightarrow> u) = (\<exists>t. s -c\<rightarrow> t \<and> t -d\<rightarrow> u)"
-by(auto elim: exec.elims intro:exec.intros)
+by(auto elim: exec.cases intro:exec.intros)
 
 lemma [iff]: "(s -IF b THEN c ELSE d\<rightarrow> t) =
               (s -if b s then c else d\<rightarrow> t)"
 apply(rule iffI)
- apply(auto elim: exec.elims intro:exec.intros)
+ apply(auto elim: exec.cases intro:exec.intros)
 apply(auto intro:exec.intros split:split_if_asm)
 done
 
 lemma [iff]: "(s -CALL p\<rightarrow> t) = (s -body p\<rightarrow> t)"
-by(blast elim: exec.elims intro:exec.intros)
+by(blast elim: exec.cases intro:exec.intros)
 
 lemma [iff]: "(s -LOCAL f; c; g\<rightarrow> u) = (\<exists>t. f s -c\<rightarrow> t \<and> u = g s t)"
-by(fastsimp elim: exec.elims intro:exec.intros)
+by(fastsimp elim: exec.cases intro:exec.intros)
 
-consts  execn    :: "(state \<times> com \<times> nat \<times> state)set"
-abbreviation
- execn' :: "state \<Rightarrow> com \<Rightarrow> nat \<Rightarrow> state \<Rightarrow> bool"   ("_/ -_-_\<rightarrow>/ _" [50,0,0,50] 50) where
- "s\<^isub>0 -c-n\<rightarrow> s\<^isub>1  \<equiv>  (s\<^isub>0,c,n,s\<^isub>1) \<in> execn"
-
-inductive execn
-intros
+inductive
+  execn :: "state \<Rightarrow> com \<Rightarrow> nat \<Rightarrow> state \<Rightarrow> bool"   ("_/ -_-_\<rightarrow>/ _" [50,0,0,50] 50)
+where
     Do:     "t \<in> f s \<Longrightarrow> s -Do f-n\<rightarrow> t"
 
-    Semi:   "\<lbrakk> s0 -c0-n\<rightarrow> s1; s1 -c1-n\<rightarrow> s2 \<rbrakk> \<Longrightarrow> s0 -c0;c1-n\<rightarrow> s2"
+  | Semi:   "\<lbrakk> s0 -c0-n\<rightarrow> s1; s1 -c1-n\<rightarrow> s2 \<rbrakk> \<Longrightarrow> s0 -c0;c1-n\<rightarrow> s2"
 
-    IfTrue: "\<lbrakk> b s; s -c0-n\<rightarrow> t \<rbrakk> \<Longrightarrow> s -IF b THEN c0 ELSE c1-n\<rightarrow> t"
+  | IfTrue: "\<lbrakk> b s; s -c0-n\<rightarrow> t \<rbrakk> \<Longrightarrow> s -IF b THEN c0 ELSE c1-n\<rightarrow> t"
 
-    IfFalse: "\<lbrakk> \<not>b s; s -c1-n\<rightarrow> t \<rbrakk> \<Longrightarrow> s -IF b THEN c0 ELSE c1-n\<rightarrow> t"
+  | IfFalse: "\<lbrakk> \<not>b s; s -c1-n\<rightarrow> t \<rbrakk> \<Longrightarrow> s -IF b THEN c0 ELSE c1-n\<rightarrow> t"
 
-    WhileFalse: "\<not>b s \<Longrightarrow> s -WHILE b DO c-n\<rightarrow> s"
+  | WhileFalse: "\<not>b s \<Longrightarrow> s -WHILE b DO c-n\<rightarrow> s"
 
-    WhileTrue:  "\<lbrakk> b s; s -c-n\<rightarrow> t; t -WHILE b DO c-n\<rightarrow> u \<rbrakk>
+  | WhileTrue:  "\<lbrakk> b s; s -c-n\<rightarrow> t; t -WHILE b DO c-n\<rightarrow> u \<rbrakk>
                 \<Longrightarrow> s -WHILE b DO c-n\<rightarrow> u"
 
-    Call:  "s -body p-n\<rightarrow> t \<Longrightarrow> s -CALL p-Suc n\<rightarrow> t"
+  | Call:  "s -body p-n\<rightarrow> t \<Longrightarrow> s -CALL p-Suc n\<rightarrow> t"
 
-    Local: "f s -c-n\<rightarrow> t \<Longrightarrow> s -LOCAL f; c; g-n\<rightarrow> g s t"
+  | Local: "f s -c-n\<rightarrow> t \<Longrightarrow> s -LOCAL f; c; g-n\<rightarrow> g s t"
 
 lemma [iff]: "(s -Do f-n\<rightarrow> t) = (t \<in> f s)"
-by(auto elim: execn.elims intro:execn.intros)
+by(auto elim: execn.cases intro:execn.intros)
 
 lemma [iff]: "(s -c1;c2-n\<rightarrow> u) = (\<exists>t. s -c1-n\<rightarrow> t \<and> t -c2-n\<rightarrow> u)"
-by(best elim: execn.elims intro:execn.intros)
+by(best elim: execn.cases intro:execn.intros)
 
 lemma [iff]: "(s -IF b THEN c ELSE d-n\<rightarrow> t) =
               (s -if b s then c else d-n\<rightarrow> t)"
 apply auto
-apply(blast elim: execn.elims intro:execn.intros)+
+apply(blast elim: execn.cases intro:execn.intros)+
 done
 
 lemma [iff]: "(s -CALL p- 0\<rightarrow> t) = False"
-by(blast elim: execn.elims intro:execn.intros)
+by(blast elim: execn.cases intro:execn.intros)
 
 lemma [iff]: "(s -CALL p-Suc n\<rightarrow> t) = (s -body p-n\<rightarrow> t)"
-by(blast elim: execn.elims intro:execn.intros)
+by(blast elim: execn.cases intro:execn.intros)
 
 lemma [iff]: "(s -LOCAL f; c; g-n\<rightarrow> u) = (\<exists>t. f s -c-n\<rightarrow> t \<and> u = g s t)"
-by(auto elim: execn.elims intro:execn.intros)
+by(auto elim: execn.cases intro:execn.intros)
 
 
 lemma exec_mono[rule_format]: "s -c-m\<rightarrow> t \<Longrightarrow> \<forall>n. m \<le> n \<longrightarrow> s -c-n\<rightarrow> t"
