thys/Abstract-Hoare-Logics/While/Termi.thy
@@ -1,5 +1,5 @@
 (*  Title:       Inductive definition of termination
-    ID:          $Id: Termi.thy,v 1.2 2006-11-17 01:28:44 makarius Exp $
+    ID:          $Id: Termi.thy,v 1.3 2007-07-11 10:05:50 stefanberghofer Exp $
     Author:      Tobias Nipkow, 2001/2006
     Maintainer:  Tobias Nipkow
 *)
@@ -8,40 +8,36 @@ theory Termi imports Lang begin
 
 subsection{*Termination*}
 
-consts  termi    :: "(com \<times> state)set"
-abbreviation
- termi' :: "com \<Rightarrow> state \<Rightarrow> bool" (infixl "\<down>" 50) where
- "c\<down>s  \<equiv>  (c,s) \<in> termi"
-
 text{*Although partial correctness appeals because of its simplicity,
 in many cases one would like the additional assurance that the command
 is guaranteed to termiate if started in a state that satisfies the
 precondition. Even to express this we need to define when a command is
 guaranteed to terminate. We can do this without modifying our existing
 semantics by merely adding a second inductively defined judgement
-@{prop"c\<down>s"} that expresses guaranteed termination of @{term c}
+@{text"c\<down>s"} that expresses guaranteed termination of @{term c}
 started in state @{term s}: *}
 
-inductive termi
-intros
+inductive
+  termi :: "com \<Rightarrow> state \<Rightarrow> bool" (infixl "\<down>" 50)
+where
   (*<*)Do[iff]:(*>*) "f s \<noteq> {} \<Longrightarrow> Do f \<down> s"
 
-  (*<*)Semi[intro!]:(*>*) "\<lbrakk> c\<^isub>1 \<down> s\<^isub>0; \<forall>s\<^isub>1. s\<^isub>0 -c\<^isub>1\<rightarrow> s\<^isub>1 \<longrightarrow> c\<^isub>2 \<down> s\<^isub>1 \<rbrakk> \<Longrightarrow> (c\<^isub>1;c\<^isub>2) \<down> s\<^isub>0"
+| (*<*)Semi[intro!]:(*>*) "\<lbrakk> c\<^isub>1 \<down> s\<^isub>0; \<forall>s\<^isub>1. s\<^isub>0 -c\<^isub>1\<rightarrow> s\<^isub>1 \<longrightarrow> c\<^isub>2 \<down> s\<^isub>1 \<rbrakk> \<Longrightarrow> (c\<^isub>1;c\<^isub>2) \<down> s\<^isub>0"
 
-  (*<*)IfT[intro,simp]:(*>*) "\<lbrakk>  b s; c\<^isub>1 \<down> s \<rbrakk> \<Longrightarrow> IF b THEN c\<^isub>1 ELSE c\<^isub>2 \<down> s"
-  (*<*)IfF[intro,simp]:(*>*) "\<lbrakk> \<not>b s; c\<^isub>2 \<down> s \<rbrakk> \<Longrightarrow> IF b THEN c\<^isub>1 ELSE c\<^isub>2 \<down> s"
+| (*<*)IfT[intro,simp]:(*>*) "\<lbrakk>  b s; c\<^isub>1 \<down> s \<rbrakk> \<Longrightarrow> IF b THEN c\<^isub>1 ELSE c\<^isub>2 \<down> s"
+| (*<*)IfF[intro,simp]:(*>*) "\<lbrakk> \<not>b s; c\<^isub>2 \<down> s \<rbrakk> \<Longrightarrow> IF b THEN c\<^isub>1 ELSE c\<^isub>2 \<down> s"
 
-  (*<*)WhileFalse:(*>*) "\<not>b s \<Longrightarrow> WHILE b DO c \<down> s"
-  (*<*)WhileTrue:(*>*) "\<lbrakk> b s; c \<down> s; \<forall>t. s -c\<rightarrow> t \<longrightarrow> WHILE b DO c \<down> t \<rbrakk> \<Longrightarrow> WHILE b DO c \<down> s"
+| (*<*)WhileFalse:(*>*) "\<not>b s \<Longrightarrow> WHILE b DO c \<down> s"
+| (*<*)WhileTrue:(*>*) "\<lbrakk> b s; c \<down> s; \<forall>t. s -c\<rightarrow> t \<longrightarrow> WHILE b DO c \<down> t \<rbrakk> \<Longrightarrow> WHILE b DO c \<down> s"
 
-  (*<*)Local:(*>*) "c \<down> f s \<Longrightarrow> LOCAL f;c;g \<down> s"
+| (*<*)Local:(*>*) "c \<down> f s \<Longrightarrow> LOCAL f;c;g \<down> s"
 
 
 lemma [iff]: "Do f \<down> s = (f s \<noteq> {})"
 apply(rule iffI)
  prefer 2
  apply(best intro:termi.intros)
-apply(erule termi.elims)
+apply(erule termi.cases)
 apply blast+
 done
 
@@ -49,7 +45,7 @@ lemma [iff]: "((c\<^isub>1;c\<^isub>2) \<down> s\<^isub>0) = (c\<^isub>1 \<down>
 apply(rule iffI)
  prefer 2
  apply(best intro:termi.intros)
-apply(erule termi.elims)
+apply(erule termi.cases)
 apply blast+
 done            
 
@@ -61,18 +57,18 @@ apply(rule impI)
 apply(rule iffI)
 prefer 2
 apply(blast intro:termi.intros)
-apply(erule termi.elims)
+apply(erule termi.cases)
 apply blast+
 apply(rule impI)
 apply(rule iffI)
 prefer 2
 apply(blast intro:termi.intros)
-apply(erule termi.elims)
+apply(erule termi.cases)
 apply blast+
 done
 
 lemma [iff]: "(LOCAL f;c;g \<down> s) = (c \<down> f s)"
-by(fast elim: termi.elims intro:termi.intros)
+by(fast elim: termi.cases intro:termi.intros)
 
 lemma termi_while_lemma[rule_format]:
  "w\<down>fk \<Longrightarrow>
